templates/lockfree/node_impl.v
@@ -21,7 +21,7 @@ Section node_impl.
         #()
       else
         let: "si" := !("succs" +ₗ "i") in
-        let: "li" := ref (#false, InjR "si") in 
+        let: "li" := ref (#false, "si") in 
         ("arr" +ₗ "i") <- "li";;
         "cN" ("i" + #1) "h" "arr" "succs".
 
@@ -69,7 +69,7 @@ Section node_impl.
         else
           "markN" "n" "i".
 
-  Definition markNode' : val :=
+  Definition markNode' : val := 
     rec: "markN" "n" "p" :=
       let: "arr" := ! ("n" +ₗ #1) in
       let: "li" := ! ("arr" +ₗ #0%nat) in
@@ -93,8 +93,8 @@ Section node_impl.
       if: (Fst "res") then
         NONEV
       else
-        if: (Snd "res") = InjR "m" then
-          let: "new" := ref (#false, InjR "m'") in
+        if: (Snd "res") = "m" then
+          let: "new" := ref (#false, "m'") in
           if: CAS ("arr" +ₗ "i") "li" "new" then
             (InjRV #())
           else
@@ -113,9 +113,7 @@ Section node_impl.
     ∗ arr ↦∗ ((fun l => # (LitLoc l)) <$> ls)
     ∗ ⌜length ls = h⌝
     ∗ ∀ (l: loc) (i: nat), ⌜ls !! i = Some l⌝ -∗
-        l ↦□ (#((mark !!! i): bool), match ((next !! i): option Node) with 
-                                        None => NONEV 
-                                      | Some ni => SOMEV #ni end).
+        l ↦□ (#((mark !!! i): bool), #((next !!! i: loc))).
 
   Definition is_array (array : loc) (xs : list Node) : iProp :=
     let vs := (fun n => # (LitLoc n)) <$> xs
@@ -152,8 +150,7 @@ Section node_impl.
          ∗ ⌜h <= length ss⌝
          ∗ ∀ (l: loc) (j: nat), 
            ⌜ls !! j = Some l⌝ -∗ ⌜j < i⌝ -∗
-             l ↦□ (#false, match ((ss !! j): option Node) with 
-                              None => NONEV | Some s => SOMEV #s end) }}}
+             l ↦□ (#false, #((ss !!! j): Node)) }}}
            createNode_rec #i #h #arr #succs
       {{{ (ls': list Node),
           RET #();
@@ -162,8 +159,7 @@ Section node_impl.
             ∗ ⌜length ls' = h⌝
             ∗ ∀ (l: loc) (j: nat), 
               ⌜ls' !! j = Some l⌝ -∗ ⌜j < h⌝ -∗
-                l ↦□ (#false, match ((ss !! j): option Node) with 
-                                  None => NONEV | Some s => SOMEV #s end) }}}.
+                l ↦□ (#false, #((ss !!! j): Node)) }}}.
   Proof.
     iIntros (Φ) "!> Hpre Hpost". iLöb as "IH" forall (i ls).
     iDestruct "Hpre" as "(Hsuccs & Harr & %Len_ls & %Hss & Hls)".
@@ -200,7 +196,7 @@ Section node_impl.
       iSplitR. by iPureIntro.
       iIntros (l' j)"%Hlj %Hj". destruct (decide (j = i)) as [-> | Hij].
       { rewrite list_lookup_insert in Hlj. inversion Hlj. subst l'.
-        rewrite Def_si. iFrame. rewrite Len_ls; lia. }
+        rewrite list_lookup_total_alt Def_si /=. iFrame. rewrite Len_ls; lia. }
       iApply "Hls". iPureIntro. rewrite list_lookup_insert_ne in Hlj; try done.
       iPureIntro; lia.
   Qed.
@@ -297,14 +293,10 @@ Section node_impl.
     iFrame "Hn Hk Harr". iSplitR. by iPureIntro.
     iModIntro. iIntros (l j)"%Hlj".
     assert (j < h) as j_lt_h. { by rewrite -Length_ls -lookup_lt_is_Some Hlj /=. }
-    rewrite lookup_total_alt Def_mark /=; try done. 
-    rewrite Def_next; try done. iSpecialize ("Hls" $! l j).
+    rewrite lookup_total_alt Def_mark /=; try done.
+    rewrite lookup_total_alt Def_next /=; try done. iSpecialize ("Hls" $! l j).
     iDestruct ("Hls" with "[%] [%]") as "H'"; try done.
-    assert (is_Some(ss !! j)) as [sj Def_sj].
-    { rewrite lookup_lt_is_Some. lia. }
-    rewrite Def_sj. apply lookup_total_correct in Def_sj.
-    rewrite -Def_sj. admit.
-  Admitted.
+  Qed.
 
   Lemma compareKey_spec (n: Node) (k': nat) :
     ⊢ <<{ ∀∀ h mark next k, node n h mark next k }>>
@@ -377,10 +369,9 @@ Section node_impl.
   Lemma findNext_spec (n: Node) (i: nat) :
     ⊢ <<{ ∀∀ h mark next k, node n h mark next k ∗ ⌜i < h⌝ }>>
           findNext #n #i @⊤
-      <<{ ∃∃ (m: bool) (opt_n': option Node),
-              node n h mark next k ∗ ⌜mark !!! i = m⌝ ∗ ⌜next !! i = opt_n'⌝ |
-              RET (match opt_n' with None => (#m, NONEV) 
-                                    | Some n' => (#m, SOMEV #n') end) }>>.
+      <<{ ∃∃ (m: bool) (n': Node),
+              node n h mark next k ∗ ⌜mark !!! i = m⌝ ∗ ⌜next !!! i = n'⌝ |
+              RET (#m, #n') }>>.
   Proof.
     iIntros (Φ) "AU".
     wp_lam. wp_pures. wp_bind (! _)%E.
@@ -401,10 +392,10 @@ Section node_impl.
     { by rewrite list_lookup_fmap Def_li /=. }
     iIntros "Harr".
     iDestruct ("Hls1" with "[%]") as "H'". apply Def_li.
-    iSpecialize ("Hclose" $! (m1 !!! i) (nx1 !! i)).
+    iSpecialize ("Hclose" $! (m1 !!! i) (nx1 !!! i)).
     iMod ("Hclose" with "[Harr]") as "HΦ".
     { iSplitL. iExists arr0, ls1. iFrame "∗#%". by iPureIntro. }
-    iModIntro. wp_pures. wp_load. wp_pures; destruct (nx1 !! i); try done.
+    iModIntro. wp_pures. wp_load. by wp_pures.
   Qed.
   
   Lemma markNode_spec (n: Node) (i: nat) :
@@ -627,18 +618,18 @@ Section node_impl.
   Qed.
 
   Lemma changeNext_spec (n m m': Node) (i: nat) :
-    ⊢  <<< ∀∀ h mark next k, node n h mark next k ∗ ⌜i < h⌝ >>>
+    ⊢  <<{ ∀∀ h mark next k, node n h mark next k ∗ ⌜i < h⌝ }>>
             changeNext #n #m #m' #i @⊤
-      <<< ∃∃ (success: bool) next',
+      <<{ ∃∃ (success: bool) next',
               node n h mark next' k
-            ∗ (match success with true => ⌜next !! i = Some m 
+            ∗ (match success with true => ⌜next !!! i = m 
                                             ∧ mark !!! i = false
                                             ∧ next' = <[i := m']> next⌝
-                                | false => ⌜(next !! i ≠ Some m ∨ 
+                                | false => ⌜(next !!! i ≠ m ∨ 
                                               mark !!! i = true)
-                                            ∧ next' = next⌝ end),
+                                            ∧ next' = next⌝ end) |
               RET (match success with true => SOMEV #() 
-                                    | false => NONEV end)  >>>.
+                                    | false => NONEV end)  }>>.
   Proof.
     iIntros (Φ) "AU". iLöb as "IH".
     wp_lam. wp_pures. wp_bind (! _)%E.
@@ -667,87 +658,74 @@ Section node_impl.
         iPureIntro; split; try done. by right. }
       iModIntro. wp_pures. wp_load. wp_pures.
       rewrite Hmi. wp_pures. done.
-    - apply not_true_is_false in Hmi.
-      destruct (nx1 !! i) as [nx1_i | ] eqn: Hnx1_i; last first.
+    - apply not_true_is_false in Hmi. rewrite Hmi.
+      destruct (decide (nx1 !!! i = m)) as [Hnx1_i | Hnx1_i]; last first.
       + iDestruct "HAU" as "[_ Hclose]".
         iSpecialize ("Hclose" $! false nx1).
         iMod ("Hclose" with "[Harr]") as "AU".
         { iSplitL. iExists arr0, ls1. iFrame "∗#%". iPureIntro.
           split; try done. by left. }
         iModIntro. wp_pures. wp_load. wp_pures.
-        rewrite Hmi. wp_pures. done.
-      + destruct (decide (nx1_i = m)) as [-> | Hnx1_i']; last first.
-        * iDestruct "HAU" as "[_ Hclose]".
-          iSpecialize ("Hclose" $! false nx1).
+        rewrite bool_decide_eq_false_2; last first. { by intros [=]. }
+        wp_pures. done.
+      + iDestruct "HAU" as "[Hclose _]".
+        iMod ("Hclose" with "[Harr]") as "AU".
+        { iSplitL; last by iPureIntro. iExists arr0, ls1. iFrame "∗#%". }
+        iModIntro. wp_pures. wp_load. wp_pures.
+        rewrite bool_decide_eq_true_2; last first. { by rewrite Hnx1_i. }
+        wp_pures. wp_alloc li_new as "Hnew". wp_pures.
+        wp_bind (CmpXchg _ _ _)%E.
+        iMod "AU" as (h2 m2 nx2 k2) "[(Node&%Hi2) HAU]".
+        iDestruct "Node" as (arr2 ls2) "(#Hk2 & #Hn2 & Harr & %Len_vs2 & #Hls2)".
+        iDestruct (mapsto_agree with "[$Hn0] [$Hn2]") as "%H'". 
+        inversion H'; subst arr2; clear H'.
+        assert (∃ li', ls2 !! i = Some li') as [li' Def_li'].
+        { apply lookup_lt_is_Some. by rewrite Len_vs2. }
+        destruct (decide (li' = li)) as [-> | Des_li].
+        * wp_apply (wp_cmpxchg_suc_offset _ _ _ _ _ _ with "[Harr]"); 
+            try done.
+          { by rewrite list_lookup_fmap Def_li' /=. }
+          { left; try done. }
+          iIntros "Harr". iDestruct "HAU" as "[_ Hclose]".
+          iSpecialize ("Hclose" $! true (<[i:=m']> nx2)).
+          iDestruct (mapsto_persist with "Hnew") as ">#Hnew'".
+          iDestruct ("Hls2" with "[%]") as "H''". apply Def_li'.
+          iDestruct (mapsto_agree with "H' H''") as "%H'". inversion H'.
+          iMod ("Hclose" with "[Harr]") as "HΦ".
+          { iSplitL. iExists arr0, (<[i:= li_new]> ls2). iFrame "#".
+            iSplitL. 
+            assert (((λ l : loc, #l) <$> <[i:=li_new]> ls2) = 
+                      <[i:=#li_new]> ((λ l : loc, #l) <$> ls2)) as ->.
+            { apply list_eq. intros i'. 
+              destruct (decide (i' = i)) as [-> | Hi'].
+              rewrite list_lookup_fmap !list_lookup_insert /=. done.
+              by rewrite fmap_length Len_vs2. by rewrite Len_vs2. 
+              rewrite list_lookup_fmap !list_lookup_insert_ne /=; try done.
+              by rewrite list_lookup_fmap. }
+            iFrame "Harr". iSplitR. { iPureIntro. by rewrite insert_length. }
+            iIntros (l j)"%Hlj". 
+            destruct (decide (j = i)) as [-> | Hj]. 
+            rewrite list_lookup_insert in Hlj. inversion Hlj. subst l.
+            rewrite -H0. 
+            assert (#((<[i:=m']> nx2 !!! i): Node) = #m') as H1'.
+            apply f_equal. by rewrite lookup_total_insert.  
+            iEval (rewrite -H1') in "Hnew'". iFrame "Hnew'". lia.
+            rewrite list_lookup_insert_ne in Hlj; try done. 
+            iClear "H' H''".
+            iDestruct ("Hls2" with "[%]") as "H'". apply Hlj. 
+            assert ((<[i:=m']> nx2 !!! j : Node) = nx2 !!! j) as H1'.
+            by rewrite lookup_total_insert_ne. iEval (rewrite -H1') in "H'". 
+            iFrame "H'". iPureIntro. repeat split; try done. by rewrite -H1. }
+          iModIntro. wp_pures. done.
+        * wp_apply (wp_cmpxchg_fail_offset _ _ _ _ _ _ #li' with "[Harr]"); 
+            try done.
+          {  by rewrite list_lookup_fmap Def_li' /=. }
+          { by intros [=->]. }
+          { left; try done. }
+          iIntros "Harr". iDestruct "HAU" as "[Hclose _]".
           iMod ("Hclose" with "[Harr]") as "AU".
-          { iSplitL. iExists arr0, ls1. iFrame "∗#%". iPureIntro.
-            split; try done. left. by intros [=]. }
-          iModIntro. wp_pures. wp_load. wp_pures.
-          rewrite Hmi. wp_pures.
-          destruct (bool_decide (InjRV #nx1_i = InjRV #m)) eqn: H'.
-          rewrite bool_decide_eq_true in H'. inversion H'; try done.
-          rewrite bool_decide_eq_false in H'.
-          wp_pures. try done.
-        * iDestruct "HAU" as "[Hclose _]".
-          iMod ("Hclose" with "[Harr]") as "AU".
-          { iSplitL; last by iPureIntro. iExists arr0, ls1. iFrame "∗#%". }
-          iModIntro. wp_pures. wp_load. wp_pures.
-          rewrite Hmi. wp_pures.
-          destruct (bool_decide (InjRV #m = InjRV #m)) eqn: H'; last first.
-          { rewrite bool_decide_eq_false in H'. exfalso; apply H'; try done. }
-          clear H'. wp_pures.
-          wp_alloc li_new as "Hnew". wp_pures.
-          wp_bind (CmpXchg _ _ _)%E.
-          iMod "AU" as (h2 m2 nx2 k2) "[(Node&%Hi2) HAU]".
-          iDestruct "Node" as (arr2 ls2) "(#Hk2 & #Hn2 & Harr & %Len_vs2 & #Hls2)".
-          iDestruct (mapsto_agree with "[$Hn0] [$Hn2]") as "%H'". 
-          inversion H'; subst arr2; clear H'.
-          assert (∃ li', ls2 !! i = Some li') as [li' Def_li'].
-          { apply lookup_lt_is_Some. by rewrite Len_vs2. }
-          destruct (decide (li' = li)) as [-> | Des_li].
-          -- wp_apply (wp_cmpxchg_suc_offset _ _ _ _ _ _ with "[Harr]"); 
-               try done.
-             { by rewrite list_lookup_fmap Def_li' /=. }
-             { left; try done. }
-             iIntros "Harr". iDestruct "HAU" as "[_ Hclose]".
-             iSpecialize ("Hclose" $! true (<[i:=m']> nx2)).
-             iDestruct (mapsto_persist with "Hnew") as ">#Hnew'".
-             iDestruct ("Hls2" with "[%]") as "H''". apply Def_li'.
-             iDestruct (mapsto_agree with "H' H''") as "%H'". inversion H'.
-             iMod ("Hclose" with "[Harr]") as "HΦ".
-             { iSplitL. iExists arr0, (<[i:= li_new]> ls2). iFrame "#".
-               iSplitL. 
-               assert (((λ l : loc, #l) <$> <[i:=li_new]> ls2) = 
-                          <[i:=#li_new]> ((λ l : loc, #l) <$> ls2)) as ->.
-               { apply list_eq. intros i'. 
-                 destruct (decide (i' = i)) as [-> | Hi'].
-                 rewrite list_lookup_fmap !list_lookup_insert /=. done.
-                 by rewrite fmap_length Len_vs2. by rewrite Len_vs2. 
-                 rewrite list_lookup_fmap !list_lookup_insert_ne /=; try done.
-                 by rewrite list_lookup_fmap. }
-               iFrame "Harr". iSplitR. { iPureIntro. by rewrite insert_length. }
-               iIntros (l j)"%Hlj". destruct (decide (j = i)) as [-> | Hj].
-               rewrite list_lookup_insert in Hlj. inversion Hlj.
-               assert (<[i:=m']> nx2 !! i = Some m') as ->. 
-               by rewrite lookup_insert. by rewrite -H0. by rewrite Len_vs2. 
-               rewrite list_lookup_insert_ne in Hlj; try done.
-               assert (<[i:=m']> nx2 !! j = nx2 !! j) as ->.
-               by rewrite lookup_insert_ne. 
-               iClear "H' H''".
-               iDestruct ("Hls2" with "[%]") as "H'". apply Hlj.
-               done.
-               iPureIntro. repeat split; try done.
-               destruct (nx2 !! i); try done. by inversion H1. }
-             iModIntro. wp_pures. done.
-          -- wp_apply (wp_cmpxchg_fail_offset _ _ _ _ _ _ #li' with "[Harr]"); 
-               try done.
-             {  by rewrite list_lookup_fmap Def_li' /=. }
-             { by intros [=->]. }
-             { left; try done. }
-             iIntros "Harr". iDestruct "HAU" as "[Hclose _]".
-             iMod ("Hclose" with "[Harr]") as "AU".
-             { iSplitL; last by iPureIntro. iExists arr0, ls2. iFrame "∗#%". }
-             iModIntro. wp_pures. by iApply "IH".
+          { iSplitL; last by iPureIntro. iExists arr0, ls2. iFrame "∗#%". }
+          iModIntro. wp_pures. by iApply "IH".
   Qed.
 
 End node_impl.
